WIP connecting to CertiRocq

theories/Compiler/correctness.v
@@ -1,8 +1,11 @@
-From Stdlib Require Import ssreflect.
-(* From Wasm Require Import binary_format_printer. *)
+From Stdlib Require Import ssreflect ssrbool.
+From Equations Require Import Equations.
 
 Require Export LambdaANF.toplevel Codegen.toplevel CodegenWasm.toplevel.
 Require Import LambdaBox_to_LambdaANF.fuel_sem.
+Require Import LambdaBox_to_LambdaANF.common.
+Require Import LambdaBox_to_LambdaANF.anf.
+Require Import LambdaBox_to_LambdaANF.anf_toplevel.
 Require Export LambdaANF.toplevel_theorems.
 Require Import compcert.lib.Maps.
 From Stdlib Require Import ZArith.
@@ -49,41 +52,126 @@ Import LambdaBox_to_LambdaANF.anf.
 Import LambdaBox_to_LambdaANF.anf_correct.
 Require Import LambdaBox_to_LambdaANF.anf_toplevel. *)
 Section lambdabox_anf_pipeline_correct.
-
+Import EGlobalEnv.
 
 Section Assumptions.
-  
-  Lemma values_glob_declared (p : EProgram.eprogram) : 
-    EWcbvEval.values_glob (wfl := final_wcbv_flags) p.1 ->
-    forall (k : kername) (decl : constant_body),
-    EGlobalEnv.declared_constant p.1 k decl -> value_decl (wfl := final_wcbv_flags) p.1 (ConstantDecl decl).
+  Print final_wcbv_flags.
+About extends.
+  Lemma value_weaken {wfl : WcbvFlags} {efl : EEnvFlags} Σ Σ' v : extends Σ Σ' -> wf_glob Σ' -> value Σ v -> value Σ' v.
   Proof.
-    destruct p as [Σ p]; cbn; clear p.
-    (* Needs weakening for value *)
+    intros hl hwf.
+    revert v. eapply value_values_ind.
+    { intros t ato; constructor 1. constructor.
+      destruct t; cbn in * => //.
+      * destruct args => //.
+        move/andP: ato => [] ->; rewrite /lookup_constructor /lookup_inductive /lookup_minductive.
+        destruct lookup_env eqn:heq => //.
+        now rewrite (hl _ _ heq). }
+    { intros p hp hp'; depelim hp. 1-4:constructor. 1-4:now constructor 2. }
+    { intros ind c mdecl idecl cdecl args wcb hl' har hargs IH.
+      eapply extends_lookup_constructor in hl'; eauto. econstructor 2; tea. }
+    { intros f args vh argsn H IH.
+      econstructor 3; tea. depelim vh.
+      eapply extends_lookup_constructor in e0; tea. econstructor; eauto.
+      econstructor. econstructor; tea. }
+  Qed.
 
-    induction 1 as [|kn d Σ HΣ IHd].
-    - intros k decl body.
-      now unfold EGlobalEnv.declared_constant.
-    - intros k decl body.
-      unfold EGlobalEnv.declared_constant in body. cbn in body.
-      move: body; case: (eqb_specT k kn) => [<-|hd]; eauto.
-      ( )
+  Lemma value_glob_lookup {fl : WcbvFlags} {efl : EEnvFlags} Σ : 
+    wf_glob Σ -> values_glob Σ -> 
+    forall kn v, EGlobalEnv.lookup_env Σ kn = Some (ConstantDecl {| cst_body := Some v |}) -> 
+    value Σ v.
+  Proof.
+    intros hwf. induction 1.
+    - intros kn v; cbn => //.
+    - intros kn' v' hl. forward IHX. now depelim hwf.
+      cbn in hl. 
+      destruct (eqb_specT kn' kn). subst kn'. noconf hl.
+      eapply value_weaken with Σ.
+      eapply EGenericMapEnv.extends_cons_wf; tea. tea.
+      now cbn in v. eapply IHX in hl.
+      eapply value_weaken; tea. now eapply EGenericMapEnv.extends_cons_wf.
+  Qed.
 
-
+  Lemma values_glob_declared Σ {efl : EEnvFlags} : 
+    wf_glob Σ ->
+    EWcbvEval.values_glob (wfl := final_wcbv_flags) Σ ->
+    forall (k : kername) (decl : constant_body),
+    declared_constant Σ k decl ->
+    value_decl (wfl := final_wcbv_flags) Σ (ConstantDecl decl).
+  Proof.
+    unfold EGlobalEnv.declared_constant.
+    intros hwf hv kn decl hl. destruct decl as [] => //.
+    destruct cst_body => //.
+    eapply value_glob_lookup in hl; tea.
+  Qed.
+  Import ETransform EImplementLazyForce EImplementBox.
   
+  Definition env_flags :=
+     let efl := EConstructorsAsBlocks.switch_cstr_as_blocks
+        (EInlineProjections.disable_projections_env_flag 
+          (ERemoveParams.switch_no_params EWellformed.all_env_flags)) in
+     let efl' := efl_coind_to_ind efl in
+     switch_off_thunk (switch_off_box efl').
 
-  Lemma values_glob_eval_env_fuel (p : EProgram.eprogram) : EWcbvEval.values_glob (wfl := final_wcbv_flags) p.1 ->
+  Definition no_primitive_flags := {|
+    has_primint := false;
+    has_primfloat := false;
+    has_primstring := false;
+    has_primarray := false; |}.
+
+  Lemma values_glob_eval_env_fuel (p : EProgram.eprogram) (efl := env_flags) :
+    wf_glob p.1 ->
+    EWcbvEval.values_glob (wfl := final_wcbv_flags) p.1 ->
     forall (k : kername) (decl : constant_body) (body : term),
     EGlobalEnv.declared_constant p.1 k decl ->
-    cst_body decl = Some body -> exists (src_v : fuel_sem.value) (f t : nat), eval_env_fuel p.1 [] body (Val src_v) f t.
+    cst_body decl = Some body -> exists (src_v : fuel_sem.value) (f t : nat), 
+    eval_env_fuel (Hf:=anf_correct.LambdaBox_resource_fuel) p.1 [] body (Val src_v) f t /\ f = <0>.
   Proof.
     destruct p as [Σ p]; cbn; clear p.
-    induction 1 as [|kn d Σ HΣ IHd].
-    - intros k decl body.
-      now unfold EGlobalEnv.declared_constant.
-    - intros k decl body. destruct d; cbn in v.
+    intros hwf hv kn decl body hd hb.
+    have hwfd := wf.wf_glob_globals_wf _ hwf _ _ _ hd hb.
+    eapply (values_glob_declared _ hwf hv) in hd; tea.
+    destruct decl as [[|]]=> //. noconf hb. cbn in hd.
+    revert t hd hwfd.
+    apply: value_values_ind.
+    { move=> t a wf. destruct t; cbn in a, wf => //.
+      do 3 eexists. split. econstructor. 2:cbn. constructor. reflexivity.
+      destruct args => //.
+      do 3 eexists. econstructor. econstructor. constructor. cbn. reflexivity. }
+    { move=> p h ih wf. cbn in wf. admit. (* no primitives supported in fuel_sem yet *) }
+    { move=> ind c mdecl idecl cdecl args wcb hlc hargs h ih.
+      cbn. move=>/andP => -[] hlc' /andP[] hlpa wfa.
+      eapply forallb_All in wfa. eapply All_mix in ih; tea.
+      assert (exists vals, Forall2 (fun t v => 
+        exists tr, eval_env_step (Hf:=anf_correct.LambdaBox_resource_fuel)
+          (Ht:=anf_correct.LambdaBox_resource_trace) Σ [] t (Val v) 0 tr) args vals).
+      { clear -ih. induction ih.
+        * exists []. constructor.
+        * destruct p as [wfx ev].
+          specialize (ev wfx). destruct ev as [srcv [f [t [ev heq]]]].
+          subst f. destruct IHih as [vals ih'].
+          exists (srcv :: vals). constructor. now exists t.
+          exact ih'. }
+      destruct H as [vals hvals].
+      assert (exists f t, eval_fuel_many (Hf := anf_correct.LambdaBox_resource_fuel) Σ [] args vals f t /\ f = 0).
+      { clear - vals hvals.
+        induction hvals.
+        - do 2 eexists. split. econstructor. reflexivity.
+        - destruct IHhvals as [f [t [ihev heq]]].
+          destruct H as [tr hv].
+          do 2 eexists. split. constructor; tea. constructor. eexact hv. cbn. subst f.
+          Print anf_correct.fuel_exp.
 
+        Print  anf_correct.fuel_resource_LambdaBox.
+        Print anf_correct.fuel_exp.
 
+      do 3 eexists. split. econstructor. reflexivity.
+      Print eval_fuel_many.
+      (* by induction *) admit. }
+    { depelim v. now cbn in e.
+      rewrite wellformed_mkApps in hwfd. now cbn in hwfd. 
+      now cbn. now cbn in y. }
+  Admitted.
 
   Context (func_tag kon_tag default_tag default_itag : positive)
           (tgm : conId_map).
@@ -104,16 +192,16 @@ Print value_decl.
     intros hp ie case_con e_tgt comp_d' cvt.
     cbn in hp.
     match goal with
-    | [ _ : EProgram.wf_eprogram ?fl p |- _ ] => set (efl := fl) in *
+    | [ _ : EProgram.wf_eprogram ?fl p /\ _ |- _ ] => set (efl := fl) in *
     end.
     unfold refines_top. unfold refines.
+    destruct hp as [wfp [vg]].
     eapply (convert_top_anf_correct func_tag kon_tag default_tag default_itag tgm (fst p) (efl:=efl)); trea.
     - (* No axioms *) cbn. admit.
     - (* If tgm came from convert_env, wouldn't that be true? *)
       admit.
-    - assert (EWcbvEval.values_glob (wfl := final_wcbv_flags) p.1). admit.
-      intros kn decl hl hb. (* The environment entries should be evaluable to values *)
-      admit.
+    - intros kn decl hl hb. (* The environment entries should be evaluable to values *)
+      eapply values_glob_eval_env_fuel; tea. apply wfp.
     - intros kn decl hl hb. (* Constants to values should carry its post-condition, for immediate values *)
       admit.
     - (* Wellformed declarations in the global environment *) 
