theories/Compiler/metarocq_pipeline.v
@@ -34,30 +34,33 @@ Program Definition certirocq_post_metarocq_pipeline econf : Transform.t global_c
   let efl := EConstructorsAsBlocks.switch_cstr_as_blocks
   (EInlineProjections.disable_projections_env_flag (ERemoveParams.switch_no_params EWellformed.all_env_flags)) in
   let efl' := efl_coind_to_ind efl in
-  let efl'' := switch_off_thunk (efl_coind_to_ind efl) in
-  let efl''' := switch_off_box (switch_off_thunk (efl_coind_to_ind efl)) in
   (* Rebuild the efficient lookup table *)
   rebuild_wf_env_transform (efl := efl) false false ▷
   (* Coinductives & cofixpoints are translated to inductive types and thunked fixpoints *)
   coinductive_to_inductive_transformation efl
-      (has_app := eq_refl) (has_rel := eq_refl) (has_pars := eq_refl) (has_cstrblocks := eq_refl) ▷
-  consts_to_values_transformation efl' final_wcbv_flags eq_refl eq_refl eq_refl ▷
+      (has_app := eq_refl) (has_rel := eq_refl) 
+      (has_pars := eq_refl) (has_cstrblocks := eq_refl) ▷
   (* Lazy-to-lambda *)
-  implement_lazy_force_transformation efl' eq_refl eq_refl eq_refl eq_refl eq_refl ▷
-  rebuild_wf_env_transform (efl := efl'') false false ▷
-  unbox_transformation efl'' final_wcbv_flags (has_app := _) (has_cofix := _) (has_prop_case := eq_refl) (has_letin := eq_refl) (has_cstrparams := eq_refl) (has_cstr_block := eq_refl) ▷
-  implement_box_transformation efl'' eq_refl eq_refl eq_refl eq_refl eq_refl ▷
+  rebuild_wf_env_transform (efl := efl') false false ▷
+  unbox_transformation efl' final_wcbv_flags (has_app := _) (has_cofix := _) (has_prop_case := eq_refl) (has_letin := eq_refl) (has_cstrparams := eq_refl) (has_cstr_block := eq_refl) ▷
   ETransform.optional_self_transform econf.(enable_unsafe).(inductives_extraction)
-    (rebuild_wf_env_transform (efl := efl''') false false ▷
-       extract_inductive_transformation efl''' final_wcbv_flags econf.(extracted_inductives) ▷
-       forget_inductive_extraction_info_transformation efl''' final_wcbv_flags) ▷
+    (rebuild_wf_env_transform (efl := efl') false false ▷
+       extract_inductive_transformation efl' final_wcbv_flags econf.(extracted_inductives) ▷
+       forget_inductive_extraction_info_transformation efl' final_wcbv_flags) ▷
   (* Heuristically do it twice for more beta-normal terms *)
   ETransform.optional_self_transform econf.(enable_unsafe).(Erasure.betared)
-    (betared_transformation efl''' final_wcbv_flags ▷
-     betared_transformation efl''' final_wcbv_flags).
+    (betared_transformation efl' final_wcbv_flags ▷
+     betared_transformation efl' final_wcbv_flags) ▷  
+  consts_to_values_transformation efl' final_wcbv_flags eq_refl eq_refl eq_refl ▷  
+  implement_lazy_force_transformation efl' eq_refl eq_refl eq_refl eq_refl eq_refl true ▷
+  implement_box_transformation (switch_off_thunk efl') eq_refl eq_refl eq_refl eq_refl eq_refl true.
 Next Obligation.
 Proof.
   destruct econf as [[? ? [] ?] ? ? ? ? ?]; cbn in *; intuition eauto.
+Qed.
+Next Obligation.
+Proof.
+  destruct econf as [[? ? [] []] ? ? [] ? []]; cbn in *; intuition eauto.
 Qed.
 Next Obligation.
 Proof.
